template-coq/theories/Primitive.v
@@ -1,6 +1,6 @@
 (* Primitive types *)
 
-From Coq Require Import Int63 PrimFloat.
+From Coq Require Import Uint63 PrimFloat.
 From MetaCoq.Template Require Import bytestring MCString.
 Local Open Scope bs.
 
@@ -10,9 +10,9 @@ Variant prim_tag :=
   (* | primArray. *)
 Derive NoConfusion EqDec for prim_tag.
 
-Definition string_of_prim_int (i:Int63.int) : string := 
+Definition string_of_prim_int (i:Uint63.int) : string := 
   (* Better? DecimalString.NilZero.string_of_uint (BinNat.N.to_uint (BinInt.Z.to_N (Int63.to_Z i))). ? *)
-  string_of_Z (Numbers.Cyclic.Int63.Uint63.to_Z i).
+  string_of_Z (Uint63.to_Z i).
 
 Definition string_of_float (f : PrimFloat.float) :=
   "<float>".
